Created has_top, has_and, & has_impl classes. Split defn of has_derives into substructural and structural parts, generalized derive_trans

src/deduction/deduction.lean
@@ -1,16 +1,46 @@
 
-class has_derives (Form : Type) :=
-  (Hyp : Type)
-  [singleHyp : has_singleton Form Hyp]
-  (derives : Hyp → Form → Prop)
-  (derive_refl : ∀ φ : Form, derives {φ} φ)
-  (derive_trans : ∀ φ ψ θ : Form, derives {φ} ψ → derives {ψ} θ → derives {φ} θ)
+namespace deduction_basic
+  class has_Hyp (Form : Type) :=
+    (Hyp : Type)
+    [emptyHyp : has_emptyc Hyp]
+    [insertHyp : has_insert Form Hyp]
+  instance singleHyp {Form : Type} [hasHyp : has_Hyp Form] : has_singleton Form hasHyp.Hyp := 
+    {singleton := λ φ, hasHyp.insertHyp.insert φ hasHyp.emptyHyp.emptyc}
+  
+  instance lawfulSingleHyp {Form : Type} [hasHyp : has_Hyp Form] : 
+  @is_lawful_singleton Form (has_Hyp.Hyp Form) hasHyp.emptyHyp hasHyp.insertHyp deduction_basic.singleHyp := 
+  { insert_emptyc_eq := begin assume φ, refl end }
 
-def der {Form : Type} [Der : has_derives Form] : Form → Form → Prop :=
-  λ φ ψ, has_derives.derives (has_derives.singleHyp.singleton φ) ψ
+  class has_derives (Form : Type) extends has_Hyp Form := 
+    (derives : Hyp → Form → Prop)
+    (derive_Trans : ∀ (Φ : Hyp) (ψ θ : Form), derives Φ ψ → derives {ψ} θ → derives Φ θ)
 
-meta def has_derives_properties {Form : Type} [Der : has_derives Form] : tactic unit :=
-  `[ apply Der.has_derives.derive_refl <|> apply Der.has_derives.derive_trans ]
+  def der {Form : Type} [Der : has_derives Form] : Form → Form → Prop :=
+    λ φ ψ, has_derives.derives {φ} ψ
 
-infix `⊢`:80 := der
+  infix `⊢`:60 := der
+
+  lemma derive_trans {Form : Type} [Der : has_derives Form] : 
+    ∀ {φ ψ θ : Form}, (φ ⊢ ψ) → (ψ ⊢ θ) → (φ ⊢ θ) :=
+  begin
+    assume φ,
+    apply Der.derive_Trans,
+  end
+
+  class has_struct_derives (Form : Type) extends has_derives Form :=
+    [memHyp : has_mem Form Hyp]
+    (inInsert : ∀ {φ : Form} {Φ : Hyp}, φ ∈ insert φ Φ)
+    (hyp : ∀ {Φ} {φ}, (φ ∈ Φ) → derives Φ φ)
+    (weak1 : ∀ {Φ} {φ} (ψ), derives Φ φ → derives (insert ψ Φ) φ)
+
+  lemma derive_refl {Form : Type} [Der : has_struct_derives Form] :
+    ∀ {φ : Form}, φ ⊢ φ :=
+  begin
+    assume φ,
+    apply Der.hyp,
+    apply Der.inInsert,
+  end
+  
+end deduction_basic
+
   
