src/deduction/deduction_cartesian.lean
@@ -1,0 +1,86 @@
+import deduction.deduction
+
+namespace deduction_cart
+
+open deduction_basic
+
+/- Truth -/
+class has_top (Form : Type) extends has_struct_derives Form := 
+  (top : Form)
+  (truth : ∀ {Φ : Hyp}, derives Φ top)
+
+notation (name:=has_top.top) `⊤`:80   := has_top.top
+
+/- Logical And -/
+class has_and (Form : Type) extends has_top Form :=
+  (and : Form → Form → Form)
+  (and_intro {Φ} {φ ψ : Form}    
+        : derives Φ φ → derives Φ ψ → derives Φ (and φ ψ))
+  (and_eliml {Φ} {φ ψ : Form}    
+        : derives Φ (and φ ψ) → derives Φ φ)
+  (and_elimr {Φ} {φ ψ : Form}    
+        : derives Φ (and φ ψ) → derives Φ ψ)
+
+infix `&`:79      := has_and.and 
+
+/- Implication -/
+class has_impl (Form : Type) extends has_and Form :=
+  (impl : Form → Form → Form)
+  (impl_intro {Φ} (φ) {ψ}   
+        : derives (insert φ Φ) ψ → derives Φ (impl φ ψ))
+  (impl_elim {Φ} (φ) {ψ} 
+        : derives Φ (impl φ ψ) → derives Φ φ → derives Φ ψ)
+
+notation (name:= has_impl.impl) φ ` ⊃ `:80 ψ := has_impl.impl φ ψ 
+
+
+/- All three -/
+end deduction_cart
+
+
+namespace cart_x
+  open deduction_basic
+  open deduction_cart
+
+  lemma and_intro1 {Form : Type} [Der : has_and Form] {φ ψ : Form} : 
+    Der.derives (Der.insertHyp.insert ψ {φ}) (φ&ψ) :=
+  begin
+    apply Der.and_intro,
+    apply Der.weak1,
+    apply derive_refl,
+    apply Der.hyp,
+    apply Der.inInsert,
+  end
+
+  lemma and_eliml1 {Form : Type} [Der : has_and Form] {φ ψ : Form} : 
+    φ & ψ ⊢ φ :=
+  begin
+    apply Der.and_eliml,
+    apply derive_refl,
+  end
+  lemma and_elimr1 {Form : Type} [Der : has_and Form] {φ ψ : Form} : 
+    φ & ψ ⊢ ψ :=
+  begin
+    apply Der.and_elimr,
+    apply derive_refl,
+  end
+
+  lemma modus_ponens {Form : Type} [Der : has_impl Form] : 
+    ∀ {φ ψ : Form}, (φ ⊃ ψ) & φ ⊢ ψ :=
+  begin
+    assume φ ψ,
+    apply Der.impl_elim φ,
+    apply and_eliml1,
+    apply and_elimr1,
+  end
+
+  lemma impl_ε {Form : Type} [Der : has_impl Form] :
+    ∀ {φ ψ θ : Form}, φ & ψ ⊢ θ  →  φ ⊢ ψ ⊃ θ :=
+  begin
+    assume φ ψ θ h,
+    apply Der.impl_intro,
+    apply Der.derive_Trans,
+    apply and_intro1,
+    exact h,
+  end
+end cart_x
